wip

theories/examples/affine.v
@@ -1,15 +1,226 @@
 (** Affine functions *)
 From Equations Require Import Equations.
+From iris.base_logic.lib Require Import na_invariants.
 From gitrees Require Import gitree program_logic.
 From gitrees.input_lang Require Import lang interp.
 From gitrees.examples Require Import store pairs.
 
+Definition s : stuckness := λ e, e = OtherError.
+
 Module io_lang.
+  Definition state := input_lang.lang.state.
   Definition ty := input_lang.lang.ty.
   Definition expr := input_lang.lang.expr.
+  Definition tyctx := tyctx ty.
   Definition typed {S} := input_lang.lang.typed (S:=S).
   Definition interp_closed {sz} (rs : gReifiers sz) `{!subReifier reify_io rs} (e : expr []) := input_lang.interp.interp_expr rs e ().
+
+Section io_lang.
+  Context {sz : nat}.
+  Variable rs : gReifiers sz.
+  Context `{!subReifier reify_io rs}.
+  Notation F := (gReifiers_ops rs).
+  Notation IT := (IT F).
+  Notation ITV := (ITV F).
+  Context `{!invGS Σ, !stateG rs Σ}.
+  Notation iProp := (iProp Σ).
+
+  Program Definition interp_tnat : ITV -n> iProp := λne αv,
+    (∃ n, αv ≡ NatV n)%I.
+  Solve All Obligations with solve_proper.
+  Program Definition interp_tarr (Φ1 Φ2 : ITV -n> iProp) := λne αv,
+    (□ ∀ σ βv, has_substate σ -∗
+               Φ1 βv -∗
+               WP@{rs} IT_of_V αv ⊙ (IT_of_V βv) @ s {{ v, ∃ σ', Φ2 v ∗ has_substate σ' }})%I.
+  Solve All Obligations with solve_proper.
+
+  Fixpoint interp_ty (τ : ty) : ITV -n> iProp :=
+    match τ with
+    | Tnat => interp_tnat
+    | Tarr τ1 τ2 => interp_tarr (interp_ty τ1) (interp_ty τ2)
+    end.
+
+  (* Definition valid1 (α : IT) (τ : ty) : iProp := *)
+  (*   (∀ σ, has_substate σ -∗ *)
+  (*         WP@{rs} α @ s {{ v, ∃ σ', interp_ty τ v ∗ has_substate σ' }}). *)
+  (* Lemma fundmanetal_closed (e : expr []) (τ : ty) : *)
+  (*   typed empC e τ → *)
+  (*   ⊢ valid1 (interp_closed rs e) τ. *)
+  (* Proof. Admitted. *)
+  Definition ssubst_valid {S} (Γ : tyctx S) (ss : ssubst S) : iProp :=
+    ([∗ list] τx ∈ zip (list_of_tyctx Γ) (list_of_ssubst (E:=F) ss),
+      interp_ty (τx.1) (τx.2))%I.
+
+  #[global] Instance io_lang_interp_ty_pers  τ βv : Persistent (io_lang.interp_ty τ βv).
+  Proof. induction τ; apply _. Qed.
+  #[global] Instance ssubst_valid_pers {S} (Γ : tyctx S) ss : Persistent (ssubst_valid  Γ  ss).
+  Proof. apply _. Qed.
+
+  Definition valid1 {S}  (Γ : tyctx S) (α : interp_scope S -n> IT) (τ : ty) : iProp :=
+    (∀ σ ss, has_substate σ -∗ ssubst_valid Γ ss -∗
+          WP@{rs} α (interp_ssubst ss) @ s {{ v, ∃ σ', interp_ty τ v ∗ has_substate σ' }}).
+
+  Lemma compat_nat {S} n (Ω : tyctx S) :
+    ⊢ valid1 Ω (interp_nat rs n) Tnat.
+  Proof.
+    iIntros (σ αs) "Hs Has".
+    simpl. iApply wp_val. iModIntro. eauto.
+  Qed.
+  Lemma compat_var {S} Ω τ (v : var S) :
+    typed_var Ω v τ →
+    ⊢ valid1 Ω (interp_var v) τ.
+  Proof.
+    intros Hv.
+    iIntros (σ ss) "Hs Has".
+    unfold ssubst_valid.
+    iInduction Hv as [|? ? ? Ω v] "IH" forall (ss); simpl.
+    - dependent elimination ss as [cons_ssubst αv ss].
+      simp list_of_tyctx list_of_ssubst interp_ssubst.
+      simp interp_var. simpl.
+      iDestruct "Has" as "[H _]".
+      iApply wp_val; eauto with iFrame.
+    - dependent elimination ss as [cons_ssubst αv ss].
+      simp list_of_tyctx list_of_ssubst interp_ssubst.
+      simp interp_var. simpl.
+      iDestruct "Has" as "[_ H]".
+      by iApply ("IH" with "Hs H").
+  Qed.
+  Lemma compat_if {S} (Γ : tyctx S) τ α β1 β2 :
+    ⊢ valid1 Γ α Tnat -∗
+      valid1 Γ β1 τ -∗
+      valid1 Γ β2 τ -∗
+      valid1 Γ (interp_if rs α β1 β2) τ.
+  Proof.
+    iIntros "H0 H1 H2".
+    iIntros (σ ss) "Hs #Has".
+    iSpecialize ("H0" with "Hs Has").
+    simpl. iApply (wp_bind _ (IFSCtx _ _)).
+    { solve_proper. }
+    iApply (wp_wand with "H0").
+    iIntros (αv) "Ha".
+    iDestruct "Ha" as (σ') "[Ha Hs]".
+    iDestruct "Ha" as (n) "Hn".
+    iModIntro. unfold IFSCtx.
+    iRewrite "Hn".
+    destruct n as [|n].
+    - rewrite IF_False; last lia.
+      iApply ("H2" with "Hs Has").
+    - rewrite IF_True; last lia.
+      iApply ("H1" with "Hs Has").
+  Qed.
+  Lemma compat_input {S} (Γ : tyctx S) :
+    ⊢ valid1 Γ (interp_input rs) Tnat.
+  Proof.
+    iIntros (σ ss) "Hs #Has".
+    simpl.
+    destruct (update_input σ) as [n σ'] eqn:Hinp.
+    iApply (wp_input with "Hs") .
+    { eauto. }
+    iNext. iIntros "_ Hs".
+    iApply wp_val. eauto with iFrame.
+  Qed.
+  Lemma compat_output {S} (Γ : tyctx S) α :
+    ⊢ valid1 Γ α Tnat → valid1 Γ (interp_output rs α) Tnat.
+  Proof.
+    iIntros "H". iIntros (σ ss) "Hs #Has".
+    simpl.
+    iApply (wp_bind _ (get_nat _)).
+    { solve_proper. }
+    iSpecialize ("H" with "Hs Has").
+    iApply (wp_wand with "H").
+    iIntros (αv) "Ha".
+    iDestruct "Ha" as (σ') "[Ha Hs]".
+    iDestruct "Ha" as (n) "Hn".
+    iModIntro. iRewrite "Hn".
+    rewrite get_nat_nat.
+    iApply (wp_output with "Hs").
+    { reflexivity. }
+    iNext. iIntros "_ Hs".
+    eauto with iFrame.
+  Qed.
+  Lemma compat_app {S} (Γ : tyctx S) α β τ1 τ2 :
+    ⊢ valid1 Γ α (Tarr τ1 τ2) -∗
+      valid1 Γ β τ1 -∗
+      valid1 Γ (interp_app rs α β) τ2.
+  Proof.
+    iIntros "H1 H2".
+    iIntros (σ ss) "Hs #Has". simpl.
+    iApply (wp_bind _  (AppRSCtx _)).
+    { solve_proper. }
+    iSpecialize ("H2" with "Hs Has").
+    iApply (wp_wand with "H2").
+    iIntros (βv) "Hb".
+    iDestruct "Hb" as (σ') "[Hb Hs]".
+    iModIntro. unfold AppRSCtx.
+    iApply (wp_bind _ (AppLSCtx (IT_of_V βv))).
+    { solve_proper. }
+    iSpecialize ("H1" with "Hs Has").
+    iApply (wp_wand with "H1").
+    iIntros (αv) "Ha".
+    iDestruct "Ha" as (σ'') "[Ha  Hs]".
+    iModIntro. unfold AppLSCtx.
+    iApply ("Ha" with "Hs Hb").
+  Qed.
+
+  Lemma compat_rec {S} (Γ : tyctx S) τ1 τ2 α :
+    ⊢ □ valid1 (consC (Tarr τ1 τ2) (consC τ1 Γ)) α τ2 -∗
+      valid1 Γ (interp_rec rs α) (Tarr τ1 τ2).
+  Proof.
+    iIntros "#H". iIntros (σ ss) "Hs #Hss".
+    pose (env := (interp_ssubst ss)). fold env.
+    simp subst_expr.
+    pose (f := (ir_unf rs α env)).
+    iAssert (interp_rec rs α env ≡ IT_of_V $ FunV (Next f))%I as "Hf".
+    { iPureIntro. apply interp_rec_unfold. }
+    iRewrite "Hf".
+    iApply wp_val. iModIntro. iExists _. iFrame.
+    iLöb as "IH". iSimpl. iModIntro.
+    clear σ.
+    iIntros (σ βv) "Hs #Hw".
+    iApply wp_lam.
+    iNext.
+    pose (ss' := cons_ssubst (FunV (Next f)) (cons_ssubst βv ss)).
+    iSpecialize ("H" $! _ ss' with "Hs []").
+    { unfold ssubst_valid.
+      unfold ss'.
+      simp list_of_tyctx list_of_ssubst.
+      by iFrame "Hw IH Hss". }
+    unfold f. simpl.
+    unfold ss'. simp interp_ssubst.
+    iAssert (IT_of_V (FunV (Next f)) ≡ interp_rec rs α env)%I as "Heq".
+    { rewrite interp_rec_unfold. done. }
+    iRewrite -"Heq". iApply "H".
+  Qed.
+  Lemma fundamental {S} (Γ : tyctx S) e τ :
+    typed Γ e τ → ⊢ valid1 Γ (interp_expr rs e) τ
+  with fundamental_val {S} (Γ : tyctx S) v τ :
+    typed_val Γ v τ → ⊢ valid1 Γ (interp_val rs v) τ.
+  Proof.
+    - destruct 1.
+      + by iApply fundamental_val.
+      + by iApply compat_var.
+      + iApply compat_rec; iApply fundamental; eauto.
+      + iApply compat_app; iApply fundamental; eauto.
+      + admit.
+      + iApply compat_if;  iApply fundamental; eauto.
+      + iApply compat_input.
+      + iApply compat_output; iApply fundamental; eauto.
+    - destruct 1.
+      + iApply compat_nat.
+      + iApply compat_rec; iApply fundamental; eauto.
+  Admitted.
+  Lemma fundmanetal_closed (e : expr []) (τ : ty) :
+    typed empC e τ →
+    ⊢ valid1 empC (interp_expr rs e) τ.
+  Proof. apply fundamental. Qed.
+
 End io_lang.
+End io_lang.
+
+#[global] Instance io_lang_interp_ty_pers {sz} (rs : gReifiers sz) `{!subReifier reify_io rs} `{!invGS Σ, !stateG rs Σ} τ βv : Persistent (io_lang.interp_ty rs τ βv).
+Proof. induction τ; apply _. Qed.
+
+
 
 Inductive ty :=
   tBool | tInt | tUnit
@@ -57,29 +268,6 @@ Inductive ty_conv : ty → input_lang.lang.ty → Type :=
 .
 
 
-Module iolang.
-  Context {sz : nat}.
-  Variable rs : gReifiers sz.
-  Context `{!subReifier reify_io rs}.
-  Notation F := (gReifiers_ops rs).
-  Notation IT := (IT F).
-  Notation ITV := (ITV F).
-  Context `{!invGS Σ, !stateG rs Σ}.
-  Notation iProp := (iProp Σ).
-
-  Variable s : stuckness.
-
-  Program Definition interp_tnat : ITV -n> iProp := λne αv,
-    (∃ n, αv ≡ NatV n)%I.
-  Solve All Obligations with solve_proper.
-  Program Definition interp_tarr (Φ1 Φ2 : ITV -n> iProp) := λne αv,
-    (□ ∀ βv, Φ1 βv -∗ WP@{rs} IT_of_V αv ⊙ (IT_of_V βv) @ s {{ Φ2 }})%I.
-  Solve All Obligations with solve_proper.
-
-End iolang.
-
-Definition s : stuckness := λ e, e = OtherError.
-
 Section affine.
   Context {sz : nat}.
   Variable rs : gReifiers sz.
@@ -98,7 +286,7 @@ Section affine.
   Program Definition thunkedV : IT -n> locO -n> ITV := λne e ℓ,
       FunV $ Next (λne _, IF (READ ℓ) (Err OtherError) (SEQ (WRITE ℓ (Nat 1)) e)).
   Solve All Obligations with first [solve_proper|solve_proper_please].
-  #[local] Instance tv_into_val e l : IntoVal (thunked e l) (thunkedV e l).
+  #[export] Instance tv_into_val e l : IntoVal (thunked e l) (thunkedV e l).
   Proof.
     unfold IntoVal. simpl. f_equiv. f_equiv. intro.
     done.
@@ -151,12 +339,21 @@ Section affine.
     | LitBool b => interp_litbool b
     | LitNat n  => interp_litnat n
     | LitUnit   => interp_litunit
-    | Var v     => interp_var v
+    | Var v     => Force ◎ interp_var v
     | Lam e    => interp_lam (interp_expr e)
     | App e1 e2 => interp_app (interp_expr e1) (interp_expr e2) ◎ interp_scope_split
     | EEmbed io_expr => constO (io_lang.interp_closed rs io_expr)
     end.
 
+
+  Context `{A:ofe}.
+  Variable (P : A → iProp).
+  Context `{!NonExpansive P}.
+
+  Program Definition expr_pred (α : IT) (Φ : ITV -n> iProp) : iProp :=
+    (∀ x : A, P x -∗ WP@{rs} α @ s {{ v, ∃ y : A, Φ v ∗ P y }}).
+  #[global] Instance expr_pred_ne : NonExpansive2 expr_pred.
+  Proof. solve_proper. Qed.
   (* interpreting tys *)
   Program Definition protected (Φ : ITV -n> iProp) : ITV -n> iProp := λne αv,
     (WP@{rs} Force (IT_of_V αv) @ s {{ Φ }})%I.
@@ -175,8 +372,7 @@ Section affine.
                        Φ1 β1v ∗ Φ2 β2v)%I.
   Solve All Obligations with solve_proper_please.
   Program Definition interp_tarr (Φ1 Φ2 : ITV -n> iProp) : ITV -n> iProp := λne αv,
-    (∀ βv, Φ1 βv -∗
-             WP@{rs} ((IT_of_V αv) ⊙ (Thunk (IT_of_V βv))) @ s {{ Φ2 }})%I.
+    (∀ βv, Φ1 βv -∗ expr_pred ((IT_of_V αv) ⊙ (Thunk (IT_of_V βv))) Φ2)%I.
   Solve All Obligations with solve_proper_please.
 
   Fixpoint interp_ty (τ : ty) : ITV -n> iProp :=
@@ -190,15 +386,16 @@ Section affine.
 
   Definition ssubst_valid {S} (Ω : tyctx S) (ss : ssubst S) : iProp :=
     ([∗ list] τx ∈ zip (list_of_tyctx Ω) (list_of_ssubst (E:=F) ss),
-      interp_ty (τx.1) (τx.2))%I.
+      protected (interp_ty (τx.1)) (τx.2))%I.
 
   Definition valid1 {S} (Ω : tyctx S) (α : interp_scope S -n> IT) (τ : ty) : iProp :=
-    ∀ ss, ssubst_valid Ω ss -∗ heap_ctx -∗ WP@{rs} α (interp_ssubst ss) @ s {{ interp_ty τ }}.
+    ∀ ss,  ssubst_valid Ω ss -∗ heap_ctx -∗ expr_pred (α (interp_ssubst ss)) (interp_ty τ).
 
   Lemma compat_bool {S} b (Ω : tyctx S) :
     ⊢ valid1 Ω (interp_litbool b) tBool.
   Proof.
     iIntros (αs) "Has #Hctx".
+    iIntros (x) "Hx".
     simpl. iApply wp_val. iModIntro.
     destruct b; simpl; eauto.
   Qed.
@@ -206,12 +403,14 @@ Section affine.
     ⊢ valid1 Ω (interp_litnat n) tInt.
   Proof.
     iIntros (αs) "Has #Hctx".
+    iIntros (x) "Hx".
     simpl. iApply wp_val. iModIntro. eauto.
   Qed.
   Lemma compat_unit {S} (Ω : tyctx S) :
     ⊢ valid1 Ω interp_litunit tUnit.
   Proof.
     iIntros (αs) "Has #Hctx".
+    iIntros (x) "Hx".
     simpl. iApply wp_val. iModIntro. eauto.
   Qed.
 
@@ -301,23 +500,58 @@ Section affine.
 
   Lemma compat_var {S} Ω τ (v : var S) :
     typed_var Ω v τ →
-    ⊢ valid1 Ω (interp_var v) τ.
+    ⊢ valid1 Ω (Force ◎ interp_var v) τ.
   Proof.
     iIntros (Hv ss) "Has #Hctx".
+    iIntros (x) "Hx".
     unfold ssubst_valid.
     iInduction Hv as [|? ? ? Ω v] "IH" forall (ss); simpl.
     - dependent elimination ss as [cons_ssubst αv ss].
       simp list_of_tyctx list_of_ssubst interp_ssubst.
       simp interp_var. simpl.
       iDestruct "Has" as "[H _]".
-      by iApply wp_val.
+      iApply (wp_wand with "H"); eauto with iFrame.
     - dependent elimination ss as [cons_ssubst αv ss].
       simp list_of_tyctx list_of_ssubst interp_ssubst.
       simp interp_var. simpl.
       iDestruct "Has" as "[_ H]".
-      iApply ("IH" with "H").
+      by iApply ("IH" with "H").
   Qed.
 
+  Equations ssubst_split {S1 S2} (αs : ssubst (E:=F) (S1++S2)) : ssubst (E:=F) S1 * ssubst (E:=F) S2 :=
+    ssubst_split (S1:=[]) αs := (emp_ssubst,αs);
+    ssubst_split (S1:=u::_) (cons_ssubst αv αs) := (cons_ssubst αv (ssubst_split αs).1, (ssubst_split αs).2).
+
+
+  Lemma ssubst_valid_app {S1 S2} (Ω1 : tyctx S1) (Ω2 : tyctx S2) αs :
+    ssubst_valid (tyctx_app Ω1 Ω2) αs ⊢ ssubst_valid Ω1 (ssubst_split αs).1
+                                      ∗ ssubst_valid Ω2 (ssubst_split αs).2.
+  Proof.
+    iInduction Ω1 as [|τ Ω1] "IH" forall (Ω2); simp tyctx_app ssubst_split.
+    - simpl. iIntros "$". unfold ssubst_valid.
+      simp list_of_ssubst list_of_tyctx. done.
+    - iIntros "H".
+      rewrite {4 5}/ssubst_valid.
+      simpl in αs.
+      dependent elimination αs as [cons_ssubst αv αs].
+      simp ssubst_split. simpl.
+      simp list_of_ssubst list_of_tyctx.
+      simpl. iDestruct "H" as "[$ H]".
+      by iApply "IH".
+  Qed.
+  Lemma interp_scope_ssubst_split {S1 S2} (αs : ssubst (S1++S2)) :
+    interp_scope_split (interp_ssubst αs) ≡
+      (interp_ssubst (ssubst_split αs).1, interp_ssubst (ssubst_split αs).2).
+  Proof.
+    induction S1 as [|u S1]; simpl.
+    - simp ssubst_split. simpl.
+      simp interp_ssubst. done.
+    - dependent elimination αs as [cons_ssubst αv αs].
+      simp ssubst_split. simpl.
+      simp interp_ssubst. repeat f_equiv; eauto; simpl.
+       + rewrite IHS1//.
+       + rewrite IHS1//.
+  Qed.
   Lemma compat_app {S1 S2} (Ω1 : tyctx S1) (Ω2 : tyctx S2)
     α β τ1 τ2 :
     ⊢ valid1 Ω1 α (tArr τ1 τ2) -∗
@@ -326,35 +560,47 @@ Section affine.
   Proof.
     iIntros "H1 H2".
     iIntros (αs) "Has #Hctx".
+    iIntros (x) "Hx".
     iEval(cbn-[interp_app]).
-    rewrite ctx_valid_split.
-    destruct (interp_ty_ctx_split αs) as [a1 a2].
+    rewrite ssubst_valid_app.
+    rewrite interp_scope_ssubst_split.
     iDestruct "Has" as "[Ha1 Ha2]". cbn-[interp_app].
-    iSpecialize ("H1" with "Ha1 Hctx").
-    iSpecialize ("H2" with "Ha2 Hctx").
+    iSpecialize ("H1"  with "Ha1 Hctx").
+    iSpecialize ("H2"  with "Ha2 Hctx").
     Local Opaque Thunk.
     iSimpl.
     iApply wp_let.
+    { solve_proper. }
+    iSpecialize ("H2" with "Hx").
     iApply (wp_wand with "H2").
     iIntros (βv) "H2".
+    iDestruct "H2" as (y) "[H2 Hy]".
     iModIntro. iSimpl.
     iApply wp_let.
+    { solve_proper. }
+    iSpecialize ("H1" with "Hy").
     iApply (wp_wand with "H1").
     iIntros (αv) "H1".
-    iModIntro. iSimpl.
-    by iApply "H1".
+    iDestruct "H1" as (z) "[H1 Hz]".
+    iModIntro. simpl.
+    iSpecialize ("H1" with "H2 Hz").
+    iApply (wp_wand with "H1"). eauto with iFrame.
   Qed.
 
-  Lemma compat_lam Ω τ1 τ2 α :
-    ⊢ valid1 (τ1::Ω) α τ2 -∗
+  Lemma compat_lam {S} (Ω : tyctx S) τ1 τ2 α :
+    ⊢ valid1 (consC τ1 Ω) α τ2 -∗
       valid1 Ω (interp_lam α) (tArr τ1 τ2).
   Proof.
     iIntros "H".
     iIntros (αs) "Has #Hctx".
+    iIntros (x) "Hx".
     iApply wp_val.
     iModIntro. simpl.
-    iIntros (βv) "Hb".
+    iExists _; iFrame.
+    iIntros (βv) "Hb". clear x.
+    iIntros (x) "Hx".
     iApply (wp_bind _ (AppRSCtx _)).
+    { solve_proper. }
     Local Transparent Thunk.
     Local Opaque thunked thunkedV.
     iSimpl. iApply (wp_alloc with "Hctx").
@@ -364,66 +610,460 @@ Section affine.
     unfold AppRSCtx.
     iApply wp_lam. iNext.
     iEval(cbn-[thunked]).
-    iApply ("H" with "[-] Hctx").
-    iSimpl. iFrame "Has".
-    iExists _.
-    rewrite IT_to_of_V. iSplit; eauto.
-    Local Transparent thunked thunkedV.
-    iApply wp_lam. iNext. simpl.
-    iApply (wp_bind _ (IFSCtx _ _)).
-    iApply (wp_read with "Hctx Hl").
-    iNext. iNext. iIntros "Hl".
-    iApply wp_val. iModIntro.
-    unfold IFSCtx. simpl.
-    rewrite IF_False; last lia.
-    iApply wp_seq.
-    { solve_proper. }
-    iApply (wp_write with "Hctx Hl").
-    iNext. iNext. iIntros "Hl".
-    iApply wp_val. iModIntro.
-    iApply "Hb".
+    iSpecialize ("H" $! (cons_ssubst (thunkedV (IT_of_V βv) l) αs)
+             with "[-Hx] Hctx Hx").
+    { unfold ssubst_valid.
+      simp list_of_ssubst list_of_tyctx. simpl.
+      iFrame.
+      Local Transparent thunked thunkedV.
+      iApply wp_lam. iNext. simpl.
+      iApply (wp_bind _ (IFSCtx _ _)).
+      iApply (wp_read with "Hctx Hl").
+      iNext. iNext. iIntros "Hl".
+      iApply wp_val. iModIntro.
+      unfold IFSCtx. simpl.
+      rewrite IF_False; last lia.
+      iApply wp_seq.
+      { solve_proper. }
+      iApply (wp_write with "Hctx Hl").
+      iNext. iNext. iIntros "Hl".
+      iApply wp_val. iModIntro.
+      iApply "Hb". }
+    simp interp_ssubst.
+    iApply "H".
   Qed.
 
+  Lemma fundamental_affine {S} (Ω : tyctx S) (e : expr S) τ :
+    typed Ω e τ →
+    ⊢ valid1 Ω (interp_expr e) τ.
+  Proof.
+    induction 1; simpl.
+    - by iApply compat_var.
+    - by iApply compat_lam.
+    - by iApply compat_app.
+    - by iApply compat_nat.
+    - by iApply compat_bool.
+    - by iApply compat_unit.
+  Qed.
 
-  Program Definition glue1_fun (glue1 glue2 : IT -n> IT) : IT -n> IT := λne α,
+End affine.
+
+Section glue.
+  Context {sz : nat}.
+  Variable rs : gReifiers sz.
+  Context `{!subReifier reify_store rs}.
+  Context `{!subReifier reify_io rs}.
+  Notation F := (gReifiers_ops rs).
+  Notation IT := (IT F).
+  Notation ITV := (ITV F).
+  Context `{!invGS Σ, !stateG rs Σ, !heapG rs Σ}.
+  Notation iProp := (iProp Σ).
+
+  Arguments Force {_ _}.
+  Arguments Thunk {_ _ _}.
+  Arguments thunked {_ _ _}.
+  Arguments thunkedV {_ _ _}.
+
+  Definition valid2 {S} (Ω : tyctx S) (α : interp_scope (E:=F) S -n> IT) (τ : ty) : iProp := valid1 rs has_substate Ω α τ.
+
+  Program Definition glue_to_affine_fun (glue_from_affine glue_to_affine : IT -n> IT) : IT -n> IT := λne α,
+    LET α $ λne α,
     λit xthnk,
       LET (Force xthnk) $ λne x,
-      LET (glue2 x) $ λne x,
-      LET (α ⊙ (Thunk x)) glue1.
+      LET (glue_from_affine x) $ λne x,
+      LET (α ⊙ (Thunk x)) glue_to_affine.
+  Solve All Obligations with solve_proper_please.
+
+  Program Definition glue_from_affine_fun (glue_from_affine glue_to_affine : IT -n> IT) : IT -n> IT := λne α,
+    LET α $ λne α,
+    LET (Thunk α) $ λne α,
+    λit xthnk,
+      LET (Force α) $ λne α,
+      LET (Force xthnk) $ λne x,
+      LET (glue_to_affine x) $ λne x,
+      LET (α ⊙ (Thunk x)) glue_from_affine.
   Solve All Obligations with solve_proper_please.
 
   Program Definition glue2_bool : IT -n> IT := λne α,
       IF α (Nat 1) (Nat 0).
 
-  Fixpoint glue1 {τ t} (conv : ty_conv τ t) : IT -n> IT :=
-    match conv with
-    | ty_conv_bool => idfun
-    | ty_conv_int  => idfun
-    | ty_conv_unit => idfun
-    | ty_conv_fun conv1 conv2 => glue1_fun (glue1 conv2) (glue2 conv1)
-    end
-  with glue2  {τ t} (conv : ty_conv τ t) : IT -n> IT :=
+  Fixpoint glue_to_affine {τ t} (conv : ty_conv τ t) : IT -n> IT :=
     match conv with
     | ty_conv_bool => glue2_bool
     | ty_conv_int  => idfun
     | ty_conv_unit => constO (Nat 0)
-    | ty_conv_fun conv1 conv2 => glue1_fun (glue1 conv1) (glue2 conv2)
+    | ty_conv_fun conv1 conv2 => glue_to_affine_fun (glue_from_affine conv1) (glue_to_affine conv2)
+    end
+  with glue_from_affine  {τ t} (conv : ty_conv τ t) : IT -n> IT :=
+    match conv with
+    | ty_conv_bool => idfun
+    | ty_conv_int  => idfun
+    | ty_conv_unit => idfun
+    | ty_conv_fun conv1 conv2 => glue_from_affine_fun (glue_from_affine conv2) (glue_to_affine conv1)
     end.
 
- 
-  Lemma compat_glue_fun (αv : ITV) (glue1 glue2 : IT -n> IT) (Φ1 Φ2 Φ1' Φ2' : ITV -n> iProp) :
-    heap_ctx ⊢
-      (∀ βv, Φ1 βv -∗ WP@{rs} glue1 (IT_of_V βv) @ s {{ x, □ Φ1' x }}) -∗
-      (∀ βv, Φ2' βv -∗ WP@{rs} glue2 (IT_of_V βv) @ s {{ Φ2 }}) -∗
-      (* (unit  →  τ1') → τ2' *)
-      □ (∀ βv, □ (WP@{rs} IT_of_V βv ⊙ (Nat 0) @ s {{ Φ1' }}) -∗
-             WP@{rs} IT_of_V αv ⊙ (IT_of_V βv) @ s {{ Φ2' }}) -∗
-      WP@{rs} glue1_fun glue2 glue1 (IT_of_V αv) @ s {{ interp_tarr Φ1 Φ2 }}.
+(* Typeclasses Opaque thunkedV. *)
+Local Opaque thunked thunkedV Thunk.
+Lemma compat_glue_to_affine_bool {S} (Ω : tyctx S) α :
+  io_lang.valid1 rs empC α Tnat ⊢
+  valid2 Ω (constO (glue2_bool (α ()))) tBool.
+Proof.
+  simpl.
+  iIntros "H". unfold io_lang.valid1.
+  iIntros (ss) "Has #Hctx". simpl.
+  iIntros (σ) "Hs".
+  iSpecialize ("H" $! _ emp_ssubst with "Hs []").
+  { unfold io_lang.ssubst_valid.
+    simp list_of_tyctx list_of_ssubst.
+    done. }
+  iApply (wp_bind _ (IFSCtx _ _)).
+  { solve_proper. }
+  iApply (wp_wand with "H").
+  iIntros (αv) "Ha". iDestruct "Ha" as (σ') "[Ha Hs]".
+  iDestruct "Ha" as (n) "Ha".
+  iRewrite "Ha".
+  unfold IFSCtx.
+  iModIntro.
+  destruct n as [|n]; simpl.
+  * rewrite IF_False ; last lia.
+    iApply wp_val; eauto with iFrame.
+  * rewrite IF_True ; last lia.
+    iApply wp_val; eauto with iFrame.
+Qed.
+Lemma compat_glue_to_affine_nat {S} (Ω : tyctx S) α :
+  io_lang.valid1 rs empC α Tnat ⊢
+  valid2 Ω (constO (α ())) tInt.
+Proof.
+  simpl.
+  iIntros "H". unfold io_lang.valid1.
+  iIntros (ss) "Has #Hctx". simpl.
+  iIntros (σ) "Hs".
+  iSpecialize ("H" $! _ emp_ssubst with "Hs []").
+  { unfold io_lang.ssubst_valid.
+    simp list_of_tyctx list_of_ssubst.
+    done. }
+  iApply (wp_wand with "H").
+  iIntros (αv) "Ha". iDestruct "Ha" as (σ') "[Ha Hs]".
+  eauto with iFrame.
+Qed.
+Lemma compat_glue_from_affine_bool α :
+  valid2 empC α tBool ⊢
+  heap_ctx -∗ io_lang.valid1 rs empC α Tnat.
+Proof.
+  simpl.
+  iIntros "H #Hctx". unfold io_lang.valid1.
+  iIntros (σ ss) "Hs Hss".
+  iSpecialize ("H" $! emp_ssubst with "[] Hctx Hs").
+  { unfold ssubst_valid.
+    simp list_of_tyctx list_of_ssubst.
+    done. }
+  dependent elimination ss as [emp_ssubst].
+  iApply (wp_wand with "H").
+  iIntros (αv) "Ha". iDestruct "Ha" as (σ') "[Ha Hs]".
+  iModIntro. iExists _; iFrame.
+  iDestruct "Ha" as "[Ha|Ha]"; iExists _; eauto.
+Qed.
+Lemma compat_glue_from_affine_nat α :
+  valid2 empC α tInt ⊢
+  heap_ctx -∗ io_lang.valid1 rs empC α Tnat.
+Proof.
+  simpl.
+  iIntros "H #Hctx". unfold io_lang.valid1.
+  iIntros (σ ss) "Hs Hss".
+  iSpecialize ("H" $! emp_ssubst with "[] Hctx Hs").
+  { unfold ssubst_valid.
+    simp list_of_tyctx list_of_ssubst.
+    done. }
+  dependent elimination ss as [emp_ssubst].
+  iApply (wp_wand with "H").
+  iIntros (αv) "Ha". iDestruct "Ha" as (σ') "[Ha Hs]".
+  iModIntro. iExists _; iFrame.
+Qed.
+Lemma compat_glue_from_affine_unit α :
+  valid2 empC α tUnit ⊢
+  heap_ctx -∗ io_lang.valid1 rs empC α Tnat.
+Proof.
+  simpl.
+  iIntros "H #Hctx". unfold io_lang.valid1.
+  iIntros (σ ss) "Hs Hss".
+  iSpecialize ("H" $! emp_ssubst with "[] Hctx Hs").
+  { unfold ssubst_valid.
+    simp list_of_tyctx list_of_ssubst.
+    done. }
+  dependent elimination ss as [emp_ssubst].
+  iApply (wp_wand with "H").
+  iIntros (αv) "Ha". iDestruct "Ha" as (σ') "[Ha Hs]".
+  iModIntro. iExists _; iFrame.
+  iExists 0. iApply "Ha".
+Qed.
+
+Lemma compat_glue_to_affine_fun {S} (Ω : tyctx S) (τ1 τ2 : ty)
+  (τ1' τ2' : io_lang.ty) α (glue_to_affine glue_from_affine : IT -n> IT) :
+  (∀ α, io_lang.valid1 rs empC α τ2'
+        ⊢ valid2 Ω (constO (glue_to_affine (α ()))) τ2) →
+  (∀ α,  valid2 empC (constO α) τ1
+        ⊢ heap_ctx -∗  io_lang.valid1 rs empC
+                               (constO (glue_from_affine α)) τ1') →
+  io_lang.valid1 rs empC α (Tarr (Tarr Tnat τ1') τ2')
+  ⊢ valid2 Ω
+      (constO (glue_to_affine_fun glue_from_affine glue_to_affine (α ())))
+      (tArr τ1 τ2).
+Proof.
+  intros G1 G2.
+  iIntros "H".
+  iIntros (αs) "Has #Hctx".
+  iIntros (σ) "Hs".
+  simpl. iApply wp_let.
+  { solve_proper. }
+  iSpecialize ("H" $! _ emp_ssubst with "Hs []").
+  { unfold io_lang.ssubst_valid.
+    simp list_of_tyctx list_of_ssubst.
+    done. }
+  iApply (wp_wand with "H").
+  iIntros (αv) "Ha". iDestruct "Ha" as (σ') "[Ha Hs]".
+  iSimpl in "Ha". iDestruct "Ha" as "#Ha".
+  iSimpl. iModIntro.
+  iApply wp_val. iModIntro.
+  simpl. iExists σ'. iFrame.
+  iIntros (βv) "Hb".
+  (* preparing a thunk *)
+  iSimpl. clear σ.
+  iIntros (σ) "Hs".
+  iApply (wp_bind _ (AppRSCtx _)).
+  { solve_proper. }
+  iApply (wp_alloc with "Hctx").
+  { solve_proper. }
+  iNext. iNext. iIntros (l) "Hl".
+  iApply wp_val. iModIntro.
+  unfold AppRSCtx.
+  iApply wp_lam. iNext.
+  iEval(cbn-[thunked]).
+  iApply wp_let.
+  { solve_proper. }
+  iApply wp_lam.
+  (* forcing a thunk *)
+  iNext. iSimpl.
+  iApply (wp_bind _ (IFSCtx _ _)).
+  { solve_proper. }
+  iApply (wp_read with "Hctx Hl").
+  iNext. iNext. iIntros "Hl".
+  iApply wp_val. iModIntro.
+  unfold IFSCtx. simpl.
+  rewrite IF_False; last lia.
+  iApply wp_seq.
+  { solve_proper. }
+  iApply (wp_write with "Hctx Hl").
+  iNext. iNext. iIntros "Hl".
+  iApply wp_val. iModIntro.
+  (* doing the glue for the argument *)
+  iApply (wp_let).
+  { solve_proper. }
+  iPoseProof (G2 (IT_of_V βv)) as "G2".
+  iSpecialize ("G2" with "[Hb]").
+  { iIntros (ss) "Hss _".
+    iIntros (σ0) "Hs". simpl.
+    iApply wp_val. eauto with iFrame. }
+  iSpecialize ("G2" with "Hctx").
+  iSpecialize ("G2" $! _ emp_ssubst with "Hs []").
+  { unfold io_lang.ssubst_valid.
+    simp list_of_tyctx list_of_ssubst.
+    done. }
+  iApply (wp_wand with "G2").
+  iIntros (β'v) "Hb". iModIntro.
+  simpl. clear σ σ'. iDestruct "Hb" as (σ) "[#Hb Hs]".
+  (* calling the original function *)
+  iApply wp_let.
+  { solve_proper. }
+  iApply (wp_bind _ (AppRSCtx _)).
+  { solve_proper. }
+  iApply (wp_alloc with "Hctx").
+  { solve_proper. }
+  iNext. iNext. iIntros (l') "Hl'".
+  iApply (wp_val _ _ (thunkedV _ _)).
+  iModIntro.
+  unfold AppRSCtx.
+  iClear "Hl". clear l.
+  iApply fupd_wp.
+  { solve_proper. }
+  iMod (inv_alloc (nroot.@"yolo") _ (∃ n, pointsto l' (Nat n)) with "[Hl']") as "#Hinv".
+  { iNext. iExists _; done. }
+  iPoseProof ("Ha" $! _ (thunkedV (IT_of_V β'v) l') with "Hs [-Has]") as "H1".
+  { iModIntro. iIntros (σ' βn) "Hs".
+    iDestruct 1 as (m) "Hbm".
+    iApply wp_lam. iNext. iSimpl.
+    iApply (wp_bind _ (IFSCtx _ _)).
+    { solve_proper. }
+    iApply (wp_read_atomic _ _ (⊤∖ nclose (nroot.@"storeE")) with "Hctx").
+    { set_solver. }
+    iInv (nroot.@"yolo") as (n) "Hl'" "Hcl".
+    iModIntro. iExists (Nat n). iFrame.
+    iNext. iNext. iIntros "Hl'".
+    iMod ("Hcl" with "[Hl']") as "_".
+    { iNext. eauto with iFrame. }
+    iModIntro. iApply wp_val.
+    iModIntro.
+    unfold IFSCtx. simpl.
+    destruct n as [|n].
+    - rewrite IF_False; last lia.
+      iApply wp_seq.
+      { solve_proper. }
+      iApply (wp_write_atomic _ _ (⊤∖ nclose (nroot.@"storeE")) with "Hctx").
+      { set_solver. }
+      iInv (nroot.@"yolo") as (n) "Hl'" "Hcl".
+      iModIntro. iExists (Nat n). iFrame.
+      iNext. iNext. iIntros "Hl'".
+      iMod ("Hcl" with "[Hl']") as "_".
+      { iNext. eauto with iFrame. }
+      iModIntro. iApply wp_val.
+      iModIntro. eauto with iFrame.
+    - rewrite IF_True; last lia.
+      iApply wp_err. done. }
+  iModIntro.
+  iApply (wp_wand with "H1").
+  iIntros (γv) "H2".
+  iModIntro. iDestruct "H2" as (σ') "[#H2 Hs]".
+  iPoseProof (G1 (constO (IT_of_V γv))) as "G1".
+  iSpecialize ("G1" with "[H2]").
+  { iIntros (σ0 ss0) "Hs Has". simpl.
+    iApply wp_val. iModIntro. eauto with iFrame. }
+  iSpecialize ("G1" with "Has Hctx Hs").
+  simpl. done.
+Qed.
+
+  Lemma glue_to_affine_compatibility {S} (Ω : tyctx S) (τ1 : ty) (τ1' : io_lang.ty)
+    (Hconv : ty_conv τ1 τ1') α :
+    io_lang.valid1 rs empC α τ1' ⊢ valid2 Ω (constO (glue_to_affine Hconv (α ()))) τ1
+  with glue_from_affine_compatibility (τ1 : ty) (τ1' : io_lang.ty)
+    (Hconv : ty_conv τ1 τ1') (α : IT) :
+    valid2 empC (constO α) τ1 ⊢ heap_ctx -∗ io_lang.valid1 rs empC (constO (glue_from_affine Hconv α)) τ1'.
+  Proof.
+    - destruct Hconv.
+      + by iApply compat_glue_to_affine_bool.
+      + by iApply compat_glue_to_affine_nat.
+      + iIntros "_".
+        simpl. iApply compat_unit.
+      + simpl. iApply compat_glue_to_affine_fun.
+        * apply glue_to_affine_compatibility.
+        * apply glue_from_affine_compatibility.
+    - destruct Hconv.
+      + iApply compat_glue_from_affine_bool.
+      + iApply compat_glue_from_affine_nat.
+      + iApply compat_glue_from_affine_unit.
+      + Opaque io_lang.interp_tarr interp_tarr.
+        iIntros "H #Hctx". iIntros (σ ss) "Hs _".
+        simpl. clear ss.
+        iSpecialize ("H" $! emp_ssubst with "[] Hctx Hs").
+        { unfold ssubst_valid. simp list_of_tyctx list_of_ssubst.
+          done. }
+        simpl.
+          simpl. iApply wp_let.
+        { solve_proper. }
+        iApply (wp_wand with "H").
+        iIntros (αv) "Ha". iDestruct "Ha" as (σ') "[Ha Hs]".
+        iSimpl in "Ha".
+        iSimpl. iModIntro.
+        iApply wp_let.
+        { solve_proper. }
+        iApply (wp_alloc with "Hctx").
+        { solve_proper_please. }
+        iNext. iNext. iIntros (l) "Hl".
+        iApply (wp_val _ _ (thunkedV _ _)). iSimpl.
+        iMod (inv_alloc (nroot.@"yolo") _
+            (pointsto l (Nat 1) ∨ (pointsto l (Nat 0) ∗ (interp_tarr rs has_substate (interp_ty rs has_substate τ1) (interp_ty rs has_substate τ2) αv))) with "[Hl Ha]") as "#Hinv".
+        { iNext. iRight. iFrame. }
+        iModIntro. iApply wp_val.
+        iModIntro. iExists _. iFrame.
+        Transparent io_lang.interp_tarr. simpl.
+        iModIntro. clear σ σ'. iIntros (σ βv) "Hs #Hb".
+        iApply wp_lam. iNext.
+        simpl.
+        iApply wp_let.
+        { solve_proper. }
+        iSpecialize ("Hb" $! _ (NatV 0) with "Hs []").
+        { eauto with iFrame. }
+        iApply wp_lam.
+        iNext. simpl.
+       iApply (wp_bind _ (IFSCtx _ _)).
+       { solve_proper_please. }
+       iApply (wp_read_atomic _ _ (⊤∖ nclose (nroot.@"storeE")) with "Hctx").
+       { set_solver. }
+       (** need thread local invariants *)
+       iInv (nroot.@"yolo") as "[Hl | [Hl Ha]]" "Hcl".
+       { iModIntro. iExists (Nat 1). iFrame.
+         iNext. iNext. iIntros "Hl".
+         iMod ("Hcl" with "[Hl]") as "_".
+         { iNext. eauto with iFrame. }
+         iModIntro. iApply wp_val.
+         iModIntro.
+         unfold IFSCtx. simpl.
+         rewrite IF_True; last lia.
+         iApply wp_err. done. }
+       iModIntro. iExists (Nat 0). iFrame.
+       iNext. iNext. iIntros "Hl".
+       iMod ("Hcl" with "[Hl]") as "_".
+       { iNext. eauto with iFrame. }
+       iModIntro. iApply wp_val.
+       iModIntro.
+       unfold IFSCtx. simpl.
+       rewrite IF_True; last lia.
+         iApp;aly wp_err. done.
+       destruct n as [|n].
+       - rewrite IF_False; last lia.
+         iApply wp_seq.
+         { solve_proper. }
+         iApply (wp_write_atomic _ _ (⊤∖ nclose (nroot.@"storeE")) with "Hctx").
+         { set_solver. }
+         iInv (nroot.@"yolo") as (n) "Hl'" "Hcl".
+         iModIntro. iExists (Nat n). iFrame.
+         iNext. iNext. iIntros "Hl'".
+         iMod ("Hcl" with "[Hl']") as "_".
+         { iNext. eauto with iFrame. }
+         iModIntro. iApply wp_val.
+         iModIntro. eauto with iFrame.
+       - rewrite IF_True; last lia.
+         iApply wp_err. done. }
+
+        iApply (wp_wand with "Hb"). clear βv.
+        iIntros (βv). iDestruct 1 as (σ') "[#Hb Hs]".
+        iModIntro. simpl.
+        iApply wp_let.
+        { solve_proper. }
+        iPoseProof (glue_to_affine_compatibility _ empC _ _ Hconv1 (IT_of_V βv)) as "G1".
+        iSpecialize ("G1" with "[Hb]").
+        { iModIntro.
+          iIntros (σ0) "Hs". simpl.
+          iApply wp_val. iModIntro. eauto with iFrame. }
+        iSpecialize ("G1" $! emp_ssubst with "[] Hctx Hs").
+        { unfold ssubst_valid. simp list_of_tyctx list_of_ssubst.
+          done. }
+        simpl.
+        iApply (wp_wand with "G1"). clear σ σ'.
+        iIntros (γv). iDestruct 1 as (σ) "[Hg Hs]".
+        iModIntro. iApply wp_let.
+        { solve_proper. }
+        iApply (wp_bind _ (AppRSCtx _)).
+        { solve_proper. }
+        iApply (wp_alloc with "Hctx").
+        { solve_proper. }
+        iNext. iNext. iIntros (l1) "Hl1".
+        iApply wp_val. unfold AppRSCtx. iModIntro.
+        iApply (wp_bind _ (AppLSCtx _)).
+  Lemma compat_glue1_fun {S} (Ω : tyctx S) (τ1 τ2 : ty)
+    (τ1' τ2' : io_lang.ty)
+    (α : IT) (glue1 glue2 : IT -n> IT) (Φ1 Φ2 Φ1' Φ2' : ITV -n> iProp) :
+    (heap_ctx ⊢ ∀ βv, interp_ty τ1 βv -∗ WP@{rs} glue1 (IT_of_V βv) @ s {{ x, □ Φ1' x }}) →
+    (heap_ctx ⊢ ∀ βv, Φ2' βv -∗ WP@{rs} glue2 (IT_of_V βv) @ s {{ interp_ty τ2 }}) →
+    (* α : (unit → τ1') → τ2' *)
+    ⊢ io_lang.valid1 α (Tarr (Tarr Tnat τ1') τ2') →
+    ⊢ valid1 Ω (constO (glue1_fun glue2 glue1 (IT_of_V αv))) (tArr τ1 τ2).
    Proof.
-     iIntros "#Hctx G1 G2 #H1".
+     intros G1 G2 Halpha.
+     iIntros (αs) "Has #Hctx".
      iApply wp_val. iModIntro.
-     iIntros (βv) "Hb".
      Local Opaque thunked thunkedV.
+     simpl.
+     iIntros (βv) "Hb".
+     (* preparing a thunk *)
      iSimpl. iApply (wp_bind _ (AppRSCtx _)).
      iApply (wp_alloc with "Hctx").
      { solve_proper. }
@@ -452,7 +1092,7 @@ Section affine.
      (* doing the glue for the argument *)
      iApply (wp_let).
      { solve_proper. }
-     iSpecialize ("G1" with "Hb").
+     iPoseProof (G1 with "Hctx Hb") as "G1".
      iApply (wp_wand with "G1").
      iIntros (β'v) "#Hb". iModIntro.
      iSimpl.
@@ -471,7 +1111,7 @@ Section affine.
      { solve_proper. }
      iMod (inv_alloc (nroot.@"yolo") _ (∃ n, pointsto l' (Nat n)) with "[Hl']") as "#Hinv".
      { iNext. iExists _; done. }
-     iSpecialize ("H1" $! (thunkedV (IT_of_V β'v) l') with "[-G2]").
+     iPoseProof (Halpha $! (thunkedV (IT_of_V β'v) l') with "[-]") as "H1".
      { iModIntro.
        iApply wp_lam. iNext. iSimpl.
        iApply (wp_bind _ (IFSCtx _ _)).
@@ -504,7 +1144,7 @@ Section affine.
      iApply (wp_wand with "H1").
      iIntros (γv) "H2".
      iModIntro.
-     by iApply "G2".
+     by iApply G2.
   Qed.
 
   Lemma compat_glue2_fun (αv : ITV) (glue1 glue2 : IT -n> IT) (Φ1 Φ2 Φ1' Φ2' : ITV -n> iProp) A :
